Code/Syntax/Signature/SubstitutionLemmas.v
@@ -1,0 +1,482 @@
+Require Import Syntax.Signature.Types.
+Require Import Syntax.Signature.Contexts.
+Require Import Syntax.Signature.Terms.
+Require Import Syntax.Signature.TermWeakenings.
+Require Import Syntax.Signature.TermSubstitutions.
+Require Import Coq.Program.Equality.
+
+(** Laws for weakenings *)
+
+(** Unitality *)
+Proposition wk_id_l
+            {B : Type}
+            {C1 C2 : Con B}
+            (w : Wk C1 C2)
+  : compWk (idWk C2) w = w.
+Proof.
+  induction w as [ | ? ? ? w IHw | ? ? ? w IHw ]
+  ; simpl ; cbn.
+  - reflexivity.
+  - rewrite IHw.
+    reflexivity.
+  - rewrite IHw.
+    reflexivity.
+Qed.
+
+Proposition wk_id_r
+            {B : Type}
+            {C1 C2 : Con B}
+            (w : Wk C1 C2)
+  : compWk w (idWk C1) = w.
+Proof.
+  induction w as [ | ? ? ? w IHw | ? ? ? w IHw ]
+  ; simpl ; cbn.
+  - reflexivity.
+  - rewrite IHw.
+    reflexivity.
+  - rewrite IHw.
+    reflexivity.
+Qed.
+
+(** Associativity *)
+Proposition wk_assoc
+            {B : Type}
+            {C1 C2 C3 C4 : Con B}
+            (w3 : Wk C3 C4)
+            (w2 : Wk C2 C3)
+            (w1 : Wk C1 C2)
+  : compWk (compWk w3 w2) w1
+    =
+    compWk w3 (compWk w2 w1).
+Proof.
+  revert w2 w3.
+  revert C3 C4.
+  induction w1 as [ | ? ? ? w1 IHw1 | ? ? ? w1 IHw1 ]
+  ; intros C3 C4 w2 w3.
+  - simpl ; cbn.
+    reflexivity.
+  - dependent induction w2 ; dependent induction w3 ; simpl ; cbn
+    ; rewrite IHw1 ; reflexivity.
+  - simpl ; cbn.
+    rewrite IHw1.
+    reflexivity.
+Qed.
+
+(** Functoriality of weakening *)
+Proposition wkVar_id
+            {B : Type}
+            {C : Con B}
+            {A : Ty B}
+            (v : Var C A)
+  : wkVar v (idWk _) = v.
+Proof.
+  induction v ; simpl ; cbn.
+  - reflexivity.
+  - rewrite IHv.
+    reflexivity.
+Qed.
+
+Proposition wkTm_id
+            {B : Type}
+            {F : Type}
+            {ar : F -> Ty B}
+            {C : Con B}
+            {A : Ty B}
+            (t : Tm ar C A)
+  : wkTm t (idWk _) = t.
+Proof.
+  induction t ; simpl.
+  - reflexivity.
+  - f_equal.
+    apply wkVar_id.
+  - f_equal.
+    exact IHt.
+  - rewrite IHt1, IHt2.
+    reflexivity.
+Qed.
+
+Proposition wkVar_comp
+            {B : Type}
+            {C1 C2 C3 : Con B}
+            {A : Ty B}
+            (v : Var C3 A)
+            (w1 : Wk C1 C2)
+            (w2 : Wk C2 C3)
+  : wkVar (wkVar v w2) w1 = wkVar v (compWk w2 w1).
+Proof.
+  revert w2 v.
+  revert C3.
+  induction w1 ; intros C3 w2 v.
+  - simpl ; cbn.
+    reflexivity.
+  - dependent induction w2.
+    + dependent induction v ; simpl ; cbn.
+      * reflexivity.
+      * f_equal.
+        apply IHw1.
+    + simpl ; cbn.
+      f_equal.
+      apply IHw1.
+  - simpl ; cbn.
+    f_equal.
+    apply IHw1.
+Qed.
+
+Proposition wkTm_comp
+            {B : Type}
+            {F : Type}
+            {ar : F -> Ty B}
+            {C1 C2 C3 : Con B}
+            {A : Ty B}
+            (t : Tm ar C3 A)
+            (w1 : Wk C1 C2)
+            (w2 : Wk C2 C3)
+  : wkTm (wkTm t w2) w1 = wkTm t (compWk w2 w1).
+Proof.
+  revert w1 w2.
+  revert C1 C2.
+  induction t ; simpl ; intros C1 C2 w1 w2.
+  - reflexivity.
+  - f_equal.
+    apply wkVar_comp.
+  - f_equal.
+    apply IHt.
+  - rewrite IHt1, IHt2.
+    reflexivity.
+Qed.
+
+(** Weakening can be written as substitution *)
+Proposition wkToSub_id
+            {B : Type}
+            {C : Con B}
+            {F : Type}
+            {ar : F -> Ty B}
+  : wkToSub (idWk C) = idSub C ar.
+Proof.
+  induction C as [ | A C IHC ].
+  - reflexivity.
+  - simpl.
+    rewrite IHC.
+    reflexivity.
+Qed.
+
+Proposition subVar_drop
+            {B : Type}
+            {C2 : Con B}
+            {A1 A2 : Ty B}
+            {F : Type}
+            {ar : F -> Ty B}
+            (v : Var C2 A1)
+            {C1 : Con B}
+            (s : Sub ar C1 C2)
+  : subVar v (dropSub A2 s)
+    =
+    subVar (Vs v) (keepSub A2 s).
+Proof.
+  induction s.
+  - reflexivity.
+  - dependent induction v ; simpl ; cbn.
+    + reflexivity.
+    + rewrite IHs.
+      reflexivity.
+Qed.
+
+Proposition subVar_keep
+            {B : Type}
+            {C2 : Con B}
+            {A1 A2 : Ty B}
+            {F : Type}
+            {ar : F -> Ty B}
+            (v : Var C2 A1)
+            {C1 : Con B}
+            (s : Sub ar C1 C2)
+  : subVar (Vs v) (keepSub A2 s)
+    =
+    wkTm (subVar v s) (Drop A2 (idWk C1)).
+Proof.
+  induction s.
+  - inversion v.
+  - dependent induction v ; simpl ; cbn.
+    + reflexivity.
+    + rewrite <- IHs.
+      apply subVar_drop.
+Qed.
+
+Proposition wkVar_is_subVar
+            {B : Type}
+            {C2 : Con B}
+            {A : Ty B}
+            {F : Type}
+            {ar : F -> Ty B}
+            (v : Var C2 A)
+            {C1 : Con B}
+            (w : Wk C1 C2)
+  : @TmVar B F ar _ _ (wkVar v w) = subVar v (wkToSub w).
+Proof.
+  induction w.
+  - inversion v.
+  - dependent induction v ; simpl ; cbn.
+    + reflexivity.
+    + rewrite subVar_drop.
+      rewrite subVar_keep.
+      simpl ; cbn.
+      rewrite <- (IHw v).
+      simpl ; cbn.
+      rewrite wkVar_id.
+      reflexivity.
+  - simpl ; cbn.
+    rewrite subVar_drop.
+    rewrite subVar_keep.
+    simpl ; cbn.
+    rewrite <- (IHw v).
+    simpl ; cbn.
+    rewrite wkVar_id.
+    reflexivity.
+Qed.
+    
+Proposition wkTm_is_subTm
+            {B : Type}
+            {C2 : Con B}
+            {A : Ty B}
+            {F : Type}
+            {ar : F -> Ty B}
+            (t : Tm ar C2 A)
+            {C1 : Con B}
+            (w : Wk C1 C2)
+  : wkTm t w = subTm t (wkToSub w).
+Proof.
+  revert w.
+  revert C1.
+  induction t ; intros C1 w ; simpl.
+  - reflexivity.
+  - apply wkVar_is_subVar.
+  - simpl.
+    rewrite IHt.
+    reflexivity.
+  - simpl.
+    rewrite IHt1.
+    rewrite IHt2.
+    reflexivity.
+Qed.
+
+(** Laws for substitution *)
+
+Proposition comp_keepSub
+            {B : Type}
+            {C1 C2 C3 : Con B}
+            {F : Type}
+            {ar : F -> Ty B}
+            {A : Ty B}
+            (s1 : Sub ar C1 C2)
+            (s2 : Sub ar C2 C3)
+  : compSub (keepSub A s2) (keepSub A s1)
+    =
+    keepSub A (compSub s2 s1).
+Proof.
+  unfold keepSub.
+  simpl ; cbn.
+  f_equal.
+  induction s2.
+  - reflexivity.
+  - simpl.
+    rewrite IHs2 ; clear IHs2.
+    f_equal.
+Admitted.
+
+Proposition subVar_comp
+            {B : Type}
+            {C3 : Con B}
+            {A : Ty B}
+            {F : Type}
+            {ar : F -> Ty B}
+            (v : Var C3 A)
+            {C1 C2 : Con B}
+            (s1 : Sub ar C1 C2)
+            (s2 : Sub ar C2 C3)
+  : subTm (subVar v s2) s1 = subVar v (compSub s2 s1).
+Proof.
+  induction s2.
+  - inversion v.
+  - dependent induction v ; simpl ; cbn.
+    + reflexivity.
+    + apply IHs2.
+Qed.
+
+Proposition subTm_comp
+            {B : Type}
+            {C3 : Con B}
+            {A : Ty B}
+            {F : Type}
+            {ar : F -> Ty B}
+            (t : Tm ar C3 A)
+            {C1 C2 : Con B}
+            (s1 : Sub ar C1 C2)
+            (s2 : Sub ar C2 C3)
+  : subTm (subTm t s2) s1 = subTm t (compSub s2 s1).
+Proof.
+  revert s2 s1.
+  revert C1 C2.
+  induction t ; simpl ; intros C1 C2 s1 s2.
+  - reflexivity.
+  - apply subVar_comp.
+  - rewrite IHt.
+    do 2 f_equal.
+    apply comp_keepSub.
+  - rewrite IHt1, IHt2.
+    reflexivity.
+Qed.
+
+Proposition subVar_id
+            {B : Type}
+            {C : Con B}
+            {A : Ty B}
+            {F : Type}
+            {ar : F -> Ty B}
+            (v : Var C A)
+  : subVar v (idSub C ar) = TmVar v.
+Proof.
+  induction C as [ | A' C IHC ].
+  - inversion v.
+  - dependent induction v ; simpl ; cbn.
+    + reflexivity.
+    + rewrite subVar_drop.
+      rewrite subVar_keep.
+      rewrite IHC.
+      simpl.
+      rewrite wkVar_id.
+      reflexivity.
+Qed.
+
+Proposition comp_drop
+            {B : Type}
+            {C1 C2 C3 : Con B}
+            {F : Type}
+            {ar : F -> Ty B}
+            (s1 : Sub ar C1 C2)
+            (s2 : Sub ar C2 C3)
+            {A : Ty B}
+            (t : Tm ar C1 A)
+  : compSub (dropSub A s2) (s1 & t) = compSub s2 s1.
+Proof.
+  induction s2.
+  - reflexivity.
+  - simpl ; cbn.
+    rewrite IHs2.
+    f_equal.
+    rewrite wkTm_is_subTm.
+    rewrite subTm_comp.
+    f_equal.
+    (*
+rewrite IHs2.
+    reflexivity.
+     *)
+Admitted.
+
+Proposition Sub_id_left
+            {B : Type}
+            {C1 C2 : Con B}
+            {F : Type}
+            {ar : F -> Ty B}
+            (s : Sub ar C1 C2)
+  : compSub (idSub _ _) s = s.
+Proof.
+  revert s.
+  revert C1.
+  induction C2 ; intros C1 s.
+  - cbn.
+    dependent induction s.
+    reflexivity.
+  - simpl.
+    dependent induction s.
+    simpl ; cbn.
+    f_equal.
+    rewrite comp_drop.
+    apply IHC2.
+Qed.
+
+Proposition Sub_id_right
+            {B : Type}
+            {C1 C2 : Con B}
+            {F : Type}
+            {ar : F -> Ty B}
+            (s : Sub ar C1 C2)
+  : compSub s (idSub _ _) = s.
+Proof.
+  induction s.
+  - reflexivity.
+  - simpl ; cbn.
+    rewrite IHs.
+    f_equal.
+    rewrite <- wkTm_id.
+    rewrite wkTm_is_subTm.
+    f_equal.
+    rewrite wkToSub_id.
+    reflexivity.
+Qed.
+
+Proposition keep_drop
+            {B : Type}
+            {C1 C2 : Con B}
+            {A : Ty B}
+            {F : Type}
+            {ar : F -> Ty B}
+            (s : Sub ar C1 C2)
+  : compSub (dropSub A s) (keepSub A (idSub C1 ar))
+    =
+    dropSub A s.
+Proof.
+  induction s ; simpl.
+  - reflexivity.
+  - rewrite IHs ; clear IHs.
+    f_equal.
+    rewrite wkTm_is_subTm.
+    rewrite subTm_comp.
+    f_equal.
+    exact (Sub_id_right (wkToSub (Drop A (idWk C1)))).
+Qed.
+
+Proposition subTm_id
+            {B : Type}
+            {C : Con B}
+            {A : Ty B}
+            {F : Type}
+            {ar : F -> Ty B}
+            (t : Tm ar C A)
+  : subTm t (idSub C ar) = t.
+Proof.
+  induction t ; simpl.
+  - reflexivity.
+  - apply subVar_id.
+  - simpl.
+    rewrite <- IHt.
+    f_equal.
+    rewrite !subTm_comp.
+    f_equal.
+    simpl ; cbn.
+    rewrite keep_drop.
+    reflexivity.
+  - rewrite IHt1, IHt2.
+    reflexivity.
+Qed.
+  
+Proposition beta_sub_help
+            {B : Type}
+            {C1 C2 : Con B}
+            {A : Ty B}
+            {F : Type}
+            {ar : F -> Ty B}
+            (t : Tm ar C2 A)
+            (w : Wk C1 C2)
+  : compSub
+      (wkToSub (Keep _ w))
+      (idSub _ _ & subTm t (wkToSub w))
+    =
+    compSub (idSub _ ar & t) (wkToSub w).
+Proof.
+  simpl ; cbn.
+  rewrite Sub_id_left.
+  f_equal.
+  rewrite comp_drop.
+  rewrite Sub_id_right.
+  reflexivity.
+Qed.
